Prove `is0_witness_closed_form` for rewritten witness
Add lemma `State.if_output`

Is0/Programs.lean
@@ -21,11 +21,21 @@ def is0_witness (input : List Felt) : List Felt :=
              , output := [42, 42]
              , constraints := []
              } <|
+    "1"         ←ₐ .Const 1;
     "x"         ←ₐ input[0];
     "isZeroBit" ←ₐ ??₀⟨"x"⟩;
     output[0]   ←ᵢ ⟨"isZeroBit"⟩;
     "invVal"    ←ₐ Inv ⟨"x"⟩;
-    output[1]   ←ᵢ ⟨"invVal"⟩
+    output[1]   ←ᵢ ⟨"invVal"⟩;
+    "arg1[0]"   ←ₐ output[0];
+    guard ⟨"arg1[0]"⟩ then
+      ?₀ ⟨"x"⟩;
+    "1 - arg1[0]" ←ₐ .Sub ⟨"1"⟩ ⟨"arg1[0]"⟩;
+    guard ⟨"1 - arg1[0]"⟩ then
+      ("arg1[1]"         ←ₐ output[1];
+      "x * arg1[1]"     ←ₐ .Mul ⟨"x"⟩ ⟨"arg1[1]"⟩;
+      "x * arg1[1] - 1" ←ₐ .Sub ⟨"x * arg1[1]"⟩ ⟨"1"⟩;
+      ?₀ ⟨"x * arg1[1] - 1"⟩)
   state'.output
 
     -- %0 = cirgen.const 1
@@ -110,7 +120,7 @@ lemma is0_constraints_closed_form {x y₁ y₂ : Felt} : is0_constraints [x] [y�
   rw [Map.update_get' 1] <;> try decide
   rw [Map.update_get' 1] <;> try decide
   rw [Map.update_get' 1] <;> try decide
-  simp
+  simp only
   rw [MLIR.run_Sequence_Assign_collapsible]
   simp only [Op.eval_andEqz, Map.update_get, Option.some.injEq, forall_apply_eq_imp_iff',
   State.update_constraint]
@@ -129,20 +139,102 @@ lemma is0_constraints_closed_form {x y₁ y₂ : Felt} : is0_constraints [x] [y�
   rw [Map.update_get' (if y₁ = 0 then True else x = 0)] <;> try decide
   simp only [Map.update_get]
 
-lemma is0_witness_closed_form {x y₁ y₂ : Felt} : is0_witness [x] = [y₁, y₂] ↔ (if x = 0 then 1 else 0) = y₁ ∧ (if x = 0 then 0 else x⁻¹) = y₂ := by
+lemma is0_witness_closed_form {x y₁ y₂ : Felt} :
+  is0_witness [x] = [y₁, y₂] ↔ (if x = 0 then 1 else 0) = y₁ ∧ (if x = 0 then 0 else x⁻¹) = y₂ := by
   unfold is0_witness
+  rw [MLIR.run_Sequence_Assign_collapsible]
+  simp only [Op.eval_const, State.update_val]
   rw [MLIR.run_Sequence_Assign_collapsible]
   simp only [Op.eval_getInput, List.getD_cons_zero, State.update_val]
   rw [MLIR.run_Sequence_Assign_collapsible]
   simp only [Op.eval_isz, Map.update_get, beq_iff_eq, State.update_val]
-  rw [MLIR.run_Sequence_Set_collapsible (if x = 0 then 1 else 0) (by simp only [Map.update_get])]
-  simp only
+  rw [MLIR.run_Sequence_Set_collapsible (if x = 0 then 1 else 0)] <;> simp only [Map.update_get]
   rw [MLIR.run_Sequence_Assign_collapsible]
   simp only [Op.eval_inv, beq_iff_eq, State.update_val]
-  rw [Map.update_update_get (by decide)]
+  rw [Map.update_get' x (by simp only) (by simp only [Map.update_get])] <;> try decide
   simp only
-  rw [MLIR.run_set]
+  rw [MLIR.run_Sequence_Set_collapsible (if x = 0 then 0 else x⁻¹)] <;> simp only [Map.update_get]
+  unfold List.set List.set ; simp only
+  rw [MLIR.run_Sequence_Assign_collapsible]
+  simp only [Op.eval_getOutput, List.getD_cons_zero, State.update_val]
+  rw [MLIR.run_Sequence_If_collapsible (if x = 0 then 1 else 0) (by simp only [Map.update_get])]
+  simp only [beq_iff_eq]
+  rw [MLIR.run_Sequence_Assign_collapsible]
+  simp only [Op.eval_sub, Map.update_get, Option.some.injEq, forall_apply_eq_imp_iff', State.update_val]
+  rw [Map.update_get' 1 (by simp only)] <;> try decide
+  swap
+  rw [Map.update_get' 1 (by simp only)] <;> try decide
+  rw [Map.update_get' 1 (by simp only)] <;> try decide
+  rw [Map.update_get' 1 (by simp only)] <;> try decide
+  simp only
+  rw [MLIR.run_If_collapsible (1 - if x = 0 then 1 else 0) (by simp only [Map.update_get])]
+  rw [MLIR.run_Sequence_Assign_collapsible]
+  simp only [beq_iff_eq, Op.eval_getOutput, List.getD_cons_succ, List.getD_cons_zero, State.update_val]
+  rw [MLIR.run_Sequence_Assign_collapsible]
+  simp only [Op.eval_mul, Map.update_get, Option.some.injEq, forall_apply_eq_imp_iff', State.update_val]
+  rw [Map.update_get' x (by simp only)] <;> try decide
+  swap
+  rw [Map.update_get' x (by simp only)] <;> try decide
+  rw [Map.update_get' x (by simp only)] <;> try decide
+  rw [Map.update_get' x (by simp only)] <;> try decide
+  rw [Map.update_get' x (by simp only)] <;> try decide
   simp only [Map.update_get]
-  unfold List.set ; unfold List.set ; simp only [List.cons.injEq, and_true]
+  simp only [mul_ite, mul_zero, ne_eq]
+  rw [MLIR.run_Sequence_Assign_collapsible]
+  simp only [Op.eval_sub, Map.update_get, Option.some.injEq, State.update_val]
+  rw [Map.update_get' 1 (by simp only)] <;> try decide
+  swap
+  rw [Map.update_get' 1 (by simp only)] <;> try decide
+  rw [Map.update_get' 1 (by simp only)] <;> try decide
+  rw [Map.update_get' 1 (by simp only)] <;> try decide
+  rw [Map.update_get' 1 (by simp only)] <;> try decide
+  rw [Map.update_get' 1 (by simp only)] <;> try decide
+  rw [Map.update_get' 1 (by simp only)] <;> try decide
+  simp only
+  rw [MLIR.run_Eqz_collapsible ((if x = 0 then 0 else x * x⁻¹) - 1) (by simp only [Map.update_get])]
+  simp only
+  rw [MLIR.run_Sequence_Eqz_collapsible x] <;> try simp only
+  swap
+  rw [Map.update_get' x (by simp only)] <;> try decide
+  rw [Map.update_get' x (by simp only)] <;> try decide
+  rw [Map.update_get' x (by simp only)] <;> try decide
+  simp only [Map.update_get]
+  rw [MLIR.run_Sequence_Assign_collapsible]
+  simp only [Op.eval_sub, Map.update_get, Option.some.injEq, forall_apply_eq_imp_iff', State.update_val]
+  rw [Map.update_get' 1 (by simp only)] <;> try decide
+  swap
+  rw [Map.update_get' 1 (by simp only)] <;> try decide
+  rw [Map.update_get' 1 (by simp only)] <;> try decide
+  rw [Map.update_get' 1 (by simp only)] <;> try decide
+  simp only
+  rw [MLIR.run_If_collapsible (1 - if x = 0 then 1 else 0) (by simp only [Map.update_get])]
+  rw [MLIR.run_Sequence_Assign_collapsible]
+  simp only [beq_iff_eq, Op.eval_getOutput, List.getD_cons_succ, List.getD_cons_zero, State.update_val]
+  rw [MLIR.run_Sequence_Assign_collapsible]
+  simp only [Op.eval_mul, Map.update_get, Option.some.injEq, forall_apply_eq_imp_iff', State.update_val]
+  rw [Map.update_get' x (by simp only)] <;> try decide
+  swap
+  rw [Map.update_get' x (by simp only)] <;> try decide
+  rw [Map.update_get' x (by simp only)] <;> try decide
+  rw [Map.update_get' x (by simp only)] <;> try decide
+  rw [Map.update_get' x (by simp only)] <;> try decide
+  simp only [Map.update_get]
+  simp only [mul_ite, mul_zero]
+  rw [MLIR.run_Sequence_Assign_collapsible]
+  simp only [Op.eval_sub, Map.update_get, Option.some.injEq, State.update_val]
+  rw [Map.update_get' 1 (by simp only)] <;> try decide
+  swap
+  rw [Map.update_get' 1 (by simp only)] <;> try decide
+  rw [Map.update_get' 1 (by simp only)] <;> try decide
+  rw [Map.update_get' 1 (by simp only)] <;> try decide
+  rw [Map.update_get' 1 (by simp only)] <;> try decide
+  rw [Map.update_get' 1 (by simp only)] <;> try decide
+  rw [Map.update_get' 1 (by simp only)] <;> try decide
+  simp only
+  rw [MLIR.run_Eqz_collapsible ((if x = 0 then 0 else x * x⁻¹) - 1) (by simp only [Map.update_get])]
+  rw [State.if_output]
+  rw [State.if_output]
+  rw [State.if_output]
+  simp only [ite_eq_right_iff, ite_self, List.cons.injEq, and_true]
 
 end Risc0
